extract most of toBits proof into lemmas

Clean/Gadgets/Bits.lean
@@ -5,16 +5,108 @@ import Clean.Gadgets.Boolean
 namespace Gadgets
 variable {p : ℕ} [prime: Fact p.Prime] [p_large_enough: Fact (p > 2)]
 
-def to_bit (x : ZMod p) : Bool := x == 1
+def to_bit (x : ZMod p) (_ : x.val = 0 ∨ x.val = 1) : Bool := x == 1
 
-def to_bits (n : ℕ) (x : ZMod p) : Vector Bool n :=
-  .ofFn fun i => x.val.testBit i
-
-def from_bits {n : ℕ} (x : Vector Bool n) : ZMod p :=
-  Nat.ofBits fun i => x[i.val]
+def from_bits {n : ℕ} (bits : Vector ℕ n) : ℕ :=
+  Fin.foldl n (fun acc ⟨i, _⟩ => acc + bits[i] * 2^i) 0
 
 def from_bits_expr {n: ℕ} (bits : Vector (Expression (F p)) n) : Expression (F p) :=
   Fin.foldl n (fun acc ⟨i, _⟩ => acc + bits[i] * (2^i : F p)) 0
+
+theorem from_bits_eval {n: ℕ} (hn : 2^n < p) {env} (bits : Vector (Expression (F p)) n)
+  (h_bits : ∀ (i : ℕ) (hi : i < n), bits[i].eval env = 0 ∨ bits[i].eval env = 1) :
+    ((from_bits_expr bits).eval env).val = from_bits (bits.map (fun b => (b.eval env).val)) := by
+
+  -- strengthen the goal for use in induction
+  suffices h_stronger :
+      ((from_bits_expr bits).eval env).val < 2^n
+      ∧ ((from_bits_expr bits).eval env).val = from_bits (bits.map (fun b => (b.eval env).val))
+    from h_stronger.right
+
+  simp only [from_bits_expr]
+
+  induction n with
+  | zero => simp only [Fin.foldl_zero, Expression.eval, ZMod.val_zero, from_bits]; simp
+  | succ n ih =>
+    simp only [Fin.foldl_succ_last, Fin.coe_castSucc, Fin.val_last, Expression.eval, from_bits,
+      Vector.getElem_map]
+    simp only [from_bits, Vector.getElem_map] at ih
+
+    -- instantiate induction hypothesis
+    have : 2*2^n < p := by rw [←Nat.pow_succ']; exact hn
+    have : 2^n < p := by linarith
+    let bits' : Vector (Expression (F p)) n := bits.pop
+    have h_bits' : ∀ j (hj : j < n), bits'[j].eval env = 0 ∨ bits'[j].eval env = 1
+      | j, hj => by
+        simp only [Vector.getElem_pop', bits']
+        exact h_bits j (Nat.lt_succ_of_lt hj)
+
+    obtain ⟨ ih_lt, ih_eq ⟩ := ih ‹_› bits' h_bits'; clear ih
+    simp only [Vector.getElem_pop', bits'] at ih_eq ih_lt
+
+    -- lift from ZMod to Nat
+    let bitn := bits[n].eval env
+    have : bitn.val < 2 := FieldUtils.boolean_lt_2 (h_bits n (Nat.lt_succ_self _))
+    have : 2 < p := p_large_enough.elim
+    have two_pow_val : ZMod.val (2 ^ n : F p) = 2 ^ n := by
+      have : @ZMod.val p 2 = 2 := ZMod.val_natCast_of_lt (by linarith)
+      rw [ZMod.val_pow, this]
+      rwa [this]
+
+    let xn : F p := Expression.eval env <| Fin.foldl n (fun acc ⟨i, _⟩ => acc + bits[i] * (2 ^ i : F p)) 0
+    have h_lt : xn.val + bitn.val * 2^n < 2^(n + 1) := by
+      have : bitn.val * 2^n ≤ 1 * 2^n := Nat.mul_le_mul_right (2 ^ n) (by linarith)
+      rw [Nat.pow_succ']
+      linarith
+
+    have h_to_nat : ZMod.val (xn + bitn * 2 ^ n) = xn.val + bitn.val * ZMod.val (2 ^ n : F p) := by
+      field_to_nat
+      rw [two_pow_val]
+      linarith
+
+    -- now we have everything in place
+    rw [h_to_nat, two_pow_val, ←ih_eq]
+    exact ⟨ h_lt, rfl ⟩
+
+theorem from_bits_testBit {n: ℕ} (bits : Vector ℕ n)
+  (h_bits : ∀ (i : ℕ) (hi : i < n), bits[i] = 0 ∨ bits[i] = 1) :
+    ∀ (i : ℕ) (hi : i < n), (from_bits bits).testBit i = (bits[i] == 1) := by
+
+  -- strengthen the goal for use in induction
+  suffices h_stronger :
+      from_bits bits < 2^n
+      ∧ ∀ (i : ℕ) (hi : i < n), (from_bits bits).testBit i = (bits[i] == 1)
+    from h_stronger.right
+
+  simp only [from_bits]
+  induction n with
+  | zero => simp_all
+  | succ n ih =>
+    simp only [Fin.foldl_succ_last, Fin.coe_castSucc, Fin.val_last]
+
+    let bits' : Vector ℕ n := bits.pop
+    have h_bits' : ∀ j (hj : j < n), bits'[j] = 0 ∨ bits'[j] = 1
+      | j, hj => by
+        simp only [Vector.getElem_pop', bits']
+        exact h_bits j (Nat.lt_succ_of_lt hj)
+
+    have h_bits_n : bits[n] = 0 ∨ bits[n] = 1 := h_bits n (Nat.lt_succ_self _)
+    obtain ⟨ ih_lt, ih_eq ⟩ := ih bits' h_bits'; clear h_bits' h_bits ih
+    simp only [Vector.getElem_pop', bits'] at ih_eq ih_lt
+
+    have : bits[n] * 2 ^ n ≤ 2^n := by
+      simp only [Nat.ofNat_pos, pow_pos, mul_le_iff_le_one_left, bits']
+      rcases h_bits_n <;> simp [*, ZMod.val_one]
+    constructor
+    · rw [Nat.pow_succ']; linarith
+
+    intro i hi
+    rw [mul_comm _ (2^n), add_comm _ (2^n * _), Nat.testBit_two_pow_mul_add _ ih_lt]
+    by_cases hin : i < n <;> simp only [hin, reduceIte]
+    · exact ih_eq i hin
+    have : n = i := by linarith
+    subst this
+    rcases h_bits_n <;> simp [*, ZMod.val_one]
 
 @[reducible] def BitVector (n : ℕ) := ProvableVector field n
 
@@ -27,7 +119,7 @@ def main {n: ℕ} (x : Expression (F p)) := do
 
   Circuit.forEach bits fun bit => assertion Boolean.circuit bit
 
-  let x' := Fin.foldl n (fun acc ⟨i, _⟩ => acc + bits[i] * (2^i : F p)) 0
+  let x' := from_bits_expr bits
   x.assert_equals x'
 
   return bits
@@ -41,7 +133,6 @@ def circuit (n : ℕ) (hn : 2^n < p) : FormalCircuit (F p) field (BitVector n) w
   local_length_eq _ _ := by simp only [main, circuit_norm, Boolean.circuit]; ac_rfl
   output_eq _ _ := by
     simp only [main, circuit_norm, Boolean.circuit, Circuit.forEach.apply_eq, var_from_offset_vector]
-    -- rfl
 
   assumptions (x : F p) := x.val < 2^n
 
@@ -61,84 +152,44 @@ def circuit (n : ℕ) (hn : 2^n < p) : FormalCircuit (F p) field (BitVector n) w
     clear h_input
 
     obtain ⟨ h_bits, h_eq ⟩ := h_holds
-    let bits i := env.get (k + i)
-    replace h_bits : ∀ (i : ℕ) (hi : i < n), bits i = 0 ∨ bits i = 1
-      | i, hi => h_bits ⟨ i, hi ⟩
 
-    have ⟨_, h_eq'⟩ : x.val < 2^n ∧ x.val = Fin.foldl n (fun acc ⟨i, _⟩ => acc + (bits i).val * 2^i) 0 := by
-      rw [congrArg ZMod.val h_eq]
-      clear h_assumptions h_eq
-      induction n with
-      | zero => simp only [Fin.foldl_zero, Expression.eval, ZMod.val_zero]; trivial
-      | succ n ih =>
-        simp only [Fin.foldl_succ_last, Fin.coe_castSucc, Fin.val_last, Expression.eval]
+    let bit_vars : Vector (Expression (F p)) n := .mapRange n fun i => var ⟨k + i⟩
+    let bits : Vector ℕ n := bit_vars.map (fun b => (b.eval env).val)
 
-        -- instantiate induction hypothesis
-        have : 2*2^n < p := by rw [←Nat.pow_succ']; exact hn
-        have : 2^n < p := by linarith
-        have h_bits' : ∀ j (hj : j < n), bits j = 0 ∨ bits j = 1
-          | j, hj => h_bits j (Nat.lt_succ_of_lt hj)
-        obtain ⟨ ih_lt, ih_eq ⟩ := ih ‹2^n < p› h_bits'; clear ih
+    have h_bit_vars : ∀ (i : ℕ) (hi : i < n), bit_vars[i].eval env = 0 ∨ bit_vars[i].eval env = 1
+      | i, hi => by
+        simp only [Vector.getElem_mapRange, bit_vars]
+        exact h_bits ⟨ i, hi ⟩
 
-        -- lift from ZMod to Nat
-        have : (bits n).val < 2 := FieldUtils.boolean_lt_2 (h_bits n (Nat.lt_succ_self _))
-        have two_pow_val : ZMod.val (2 ^ n : F p) = 2 ^ n := by
-          have : @ZMod.val p 2 = 2 := ZMod.val_natCast_of_lt (by linarith [p_large_enough.elim])
-          rw [ZMod.val_pow, this]
-          rwa [this]
-        let xn : F p := Expression.eval env <| Fin.foldl n (fun acc ⟨i, _⟩ => acc + var (F:=F p) ⟨ k + i ⟩ * (2 ^ i : F p)) 0
-        have h_lt : xn.val + (bits n).val * 2^n < 2^(n + 1) := by
-          have : (env.get (k + n)).val * 2^n ≤ 1 * 2^n := Nat.mul_le_mul_right (2 ^ n) (by linarith)
-          rw [Nat.pow_succ']
-          linarith
-        have h_to_nat : ZMod.val (xn + (bits n) * 2 ^ n) = xn.val + (bits n).val * ZMod.val (2 ^ n : F p) := by
-          field_to_nat
-          rw [two_pow_val]
-          linarith
+    replace h_bits : ∀ (i : ℕ) (hi : i < n), bits[i] = 0 ∨ bits[i] = 1
+      | i, hi => by
+        simp only [Vector.getElem_map, bits]
+        rcases h_bit_vars i hi with h|h
+        · left; rw [h, ZMod.val_zero]
+        · right; rw [h, ZMod.val_one]
 
-        -- now we have everything in place
-        rw [h_to_nat, two_pow_val, ←ih_eq]
-        exact ⟨ h_lt, rfl ⟩
-
-    have ⟨_, h_testbit⟩ : x.val < 2^n ∧ ∀ {i : ℕ} (hi : i < n), x.val.testBit i = ((bits i).val == 1) := by
-      rw [h_eq']
-      clear h_assumptions h_eq h_eq' ‹ZMod.val x < 2 ^ n› hn
-      simp only
-      induction n with
-      | zero =>
-        simp only [Fin.foldl_zero]
-        exact ⟨ by trivial, fun i => by trivial ⟩
-      | succ n ih =>
-        simp only [Fin.foldl_succ_last, Fin.coe_castSucc, Fin.val_last]
-        have h_bits_prev : ∀ j (hj : j < n), bits j = 0 ∨ bits j = 1
-          | j, hj => h_bits j (Nat.lt_succ_of_lt hj)
-        have h_bits_n : bits n = 0 ∨ bits n = 1 := h_bits n (Nat.lt_succ_self _)
-        obtain ⟨ ih_lt, ih_eq ⟩ := ih h_bits_prev; clear h_bits_prev h_bits ih
-        have : 2 ^ n * ZMod.val (bits n) ≤ 2^n := by
-          simp only [Nat.ofNat_pos, pow_pos, mul_le_iff_le_one_right]
-          rcases h_bits_n <;> simp [*, ZMod.val_one]
-        constructor
-        · rw [Nat.pow_succ']; linarith
-        intro i hi
-        rw [mul_comm _ (2^n), add_comm _ (2^n * _), Nat.testBit_two_pow_mul_add _ ih_lt]
-        by_cases hin : i < n <;> simp only [hin, reduceIte]
-        · exact ih_eq hin
-        have : n = i := by linarith
-        subst this
-        rcases h_bits_n <;> simp [*, ZMod.val_one]
-
+    change x = (from_bits_expr bit_vars).eval env at h_eq
+    rw [h_eq, from_bits_eval hn bit_vars h_bit_vars]
     intro i hi
+
+    show env.get (k + i) = if (from_bits bits).testBit i then 1 else 0
+
+    have h_bit_i : (env.get (k + i)).val = bits[i] := by
+      simp [Vector.getElem_map, bits, bit_vars, Expression.eval]
+    apply FieldUtils.ext
+    rw [h_bit_i, from_bits_testBit bits h_bits i hi]
     specialize h_bits i hi
-    simp only at h_bits
-    rw [h_testbit hi]
-    simp only [beq_iff_eq]
-    rcases h_bits with h|h
-    · simp [h, bits]
-    · simp [h, bits, ZMod.val_one]
+    rcases h_bits <;> simp [*, bits, ZMod.val_one]
 
   completeness := by
     intro k env x_var h_env x h_input h_assumptions
-    simp only [main, circuit_norm, eval_vector, var_from_offset_vector] at *
+    simp only [main, circuit_norm, Boolean.circuit, eval_vector, var_from_offset_vector, from_bits_expr] at *
+    split
+    · rename_i h_eq
+      obtain rfl : n = 0 := Circuit.forEach.no_empty h_eq
+      simp_all [Expression.eval]
+    rename_i h_eq; clear h_eq
+    simp only [h_input, circuit_norm, subcircuit_norm, true_implies, true_and, and_true] at h_env ⊢
     sorry
 
 end Gadgets.ToBits
